\documentclass[12pt, english]{article}
%----------------------------------------
\usepackage[a4paper, top=1cm, bottom=2cm]{geometry}
\usepackage{graphicx, xcolor}
\usepackage{amssymb,amsmath}
\usepackage{url}
\definecolor{mygray}{rgb}{0.9,0.9,0.9}
\definecolor{mygreen}{rgb}{0,0.6,0}

\usepackage{listings}
\lstset{ 
  backgroundcolor=\color{mygray},
  basicstyle=\ttfamily\footnotesize,
  breaklines=true,
  commentstyle=\color{mygreen},
  deletekeywords={...},
  escapeinside={\%*}{*)},
  frame=single,
  showstringspaces=false,
  language=Python
}
\usepackage[many]{tcolorbox}
\tcbuselibrary{breakable}

\input{macros.tex}

%----------------------------------------
\title{Finite difference}
\author{Roland Becker}

%==========================================
\begin{document}
%==========================================
\maketitle
%
%
%==========================================
\section{Grid}\label{sec:}
%==========================================
%
%
\begin{equation}\label{eq:}
x_{n+1} = x_n + \omega w_n,\quad  w_n = B r_n, \quad r_n := b - A x_n
\end{equation}
%
If $A$ is SPD, we can either minimize with respect to the norm $\norm{A\cdot}$ or $\norm{A^{\frac12}\cdot}$
%
\begin{align*}
\omega^{(1)} = \frac{\transpose{r_n}{Aw_n}}{\transpose{(Aw_n)}{Aw_n}},\quad
\omega^{(2)} = \frac{\transpose{r_n}{w_n}}{\transpose{(Aw_n)}{w_n}}
\end{align*}
%
If $A$ is not symmetric, $\omega^{(2)}$ is still be well defined, if $A$ is elliptic ($\transpose{\xi}A\xi\ge \alpha\transpose{\xi}\xi$) and corresponds to minimization over the space $\vect{x_n, w_n}$.

Now let us consider a Gauss-Seidel-type iteration with $A=L+U$ and
%
\begin{align*}
x_{n+1} = (1-\omega)x_n + \omega L^{-1}(b- U x^n) = x_n +  \omega L^{-1}r^n.
\end{align*}
%


%
%==========================================
\section{Mixed FEM}\label{sec:}
%==========================================
%

%
%==========================================
\section{Grid}\label{sec:}
%==========================================
%
We suppose the following numbering
%
\begin{equation}\label{eq:}
ii = \sum_{j=0}^{d-1}\left(\prod_{k=j+1}^{d-1}n_k\right) i_j,\quad i=[i_0,\ldots,i_{d-1}]
\end{equation}
%
%
%
%==========================================
\section{Mixed FEM}\label{sec:}
%==========================================
%
The mixed formulation on a $d$-dimensional brick leads to
%
\begin{equation}\label{eq:structfemsys}
\begin{bmatrix}
A_1 && &  & B_1 \\
 & A_2 &&  & B_2 \\
&&\ddots&&\vdots  \\
& &  &  A_d& B_d \\
C_1 & C_2 &\cdots & C_d & D
\end{bmatrix}
\begin{bmatrix}
  u_1 \\ u_2 \\ \vdots \\ u_d \\ p
\end{bmatrix}
=
\begin{bmatrix}
  g_1 \\ g_2 \\ \vdots \\ g_d \\ f
\end{bmatrix}
\end{equation}
which leads to the pressure equation
\begin{equation}\label{eq:structfemsys}
  S p = f - \sum_{i=1}^d C_i A_i^{-1} g_i,\quad S := D - \sum_{i=1}^d C_i A_i^{-1}B_i
\end{equation}
  which allows to recover the fluxes by
\begin{equation*}
  A_i u_i = g_i  - B_i p.
\end{equation*}

%
%~~~~~~~~~~~~~~~~~~~~~~~~~~~~~
\subsubsection{Elimination in $d=1$}
%~~~~~~~~~~~~~~~~~~~~~~~~~~~~~
%
We have the following equations
%
\begin{equation}\label{eq:}
%
\left\{
\begin{aligned}
a_{i,i-1} u_{i-1} + a_{i,i} u_{i} + a_{i,i+1} u_{i+1} + b_{i,i-\frac12} p_{i-\frac12}   + b_{i,i+\frac12} p_{i+\frac12} =& g_i\\
c_{i-\frac12, i-1} u_{i-1} + c_{i-\frac12, i} u_{i} =& f_{i-\frac12}\\
c_{i+\frac12, i} u_{i} + c_{i+\frac12, i+1} u_{i+1} =& f_{i+\frac12}
\end{aligned}
\right.
%
\end{equation}
%
We can use the last two equations to eliminate $u_{i\pm1}$, thus
%
\begin{equation}\label{eq:}
x_i u_i =  g_i - \frac{a_{i,i-1}}{c_{i-\frac12, i-1}}f_{i-\frac12}- \frac{a_{i,i+1}}{c_{i+\frac12, i+1}}f_{i+\frac12}
- b_{i,i-\frac12} p_{i-\frac12}   - b_{i,i+\frac12} p_{i+\frac12},\quad
x_i = a_{i,i} - \frac{a_{i,i-1}c_{i-\frac12, i}}{c_{i-\frac12, i-1}}- \frac{a_{i,i+1}c_{i+\frac12, i}}{c_{i+\frac12, i+1}}
\end{equation}
%
For a boundary node we have, say the left, $i=0$, we have
\begin{equation}\label{eq:}
%
\left\{
\begin{aligned}
a_{0,0} u_{0} + a_{0,1} u_{1} + b_{0,\frac12} p_{\frac12} =& g_0\\
c_{\frac12, 0} u_{0} + c_{\frac12, 1} u_{1} =& f_{\frac12}
\end{aligned}
\right.
%
\end{equation}
%
Using the last  equation to eliminate $u_{1}$, thus
%
\begin{equation}\label{eq:}
x_0 u_0 =  g_0 - \frac{a_{0,1}}{c_{\frac12, 1}}f_{\frac12}
  - b_{0,\frac12} p_{\frac12},\quad
x_0 = a_{0,0} -  \frac{a_{0,1}c_{\frac12, 0}}{c_{\frac12, 1}}
\end{equation}
%
This gives the following finite difference stencil on the boundary
%
%
\begin{align*}
\frac{c_{\frac12, 0}}{x_{0}} \left(g_0 - \frac{a_{0,1}}{c_{\frac12, 1}}f_{\frac12}
  - b_{0,\frac12} p_{\frac12}\right) 
  + \frac{c_{\frac12, 1}}{x_1} \left(
  g_1 - \frac{a_{1,0}}{c_{\frac12, 0}}f_{\frac12}- \frac{a_{1,2}}{c_{\frac32, 2}}f_{\frac32}
- b_{1,\frac12} p_{\frac12}   - b_{1,\frac32} p_{\frac32}
\right) =& f_{\frac12}
\end{align*}
%
and on the interior
%
\begin{align*}
&\frac{c_{i+\frac12, i}}{x_i} \left( 
g_i - \frac{a_{i,i-1}}{c_{i-\frac12, i-1}}f_{i-\frac12}- \frac{a_{i,i+1}}{c_{i+\frac12, i+1}}f_{i+\frac12}
- b_{i,i-\frac12} p_{i-\frac12}   - b_{i,i+\frac12} p_{i+\frac12}
\right)  
\\+& \frac{c_{i+\frac12, i+1}}{x_{i+1}} \left( 
g_{i+1} - \frac{a_{i+1,i}}{c_{i+\frac12, i}}f_{i+\frac12}- \frac{a_{i+1,i+1+1}}{c_{i+\frac32, i+1+1}}f_{i+\frac32}
- b_{i+1,i+\frac12} p_{i+\frac12}   - b_{i+1,i+\frac32} p_{i+\frac32}
\right) =& f_{i+\frac12}
\end{align*}
%

\begin{equation}\label{eq:}
%
\left\{
\begin{aligned}
\end{aligned}
\right.
%
\end{equation}
%


%==========================================
\end{document}  
%==========================================
